deps/poulet4/lib/P4automata/Bisimulations/WPLeaps.v
@@ -31,9 +31,8 @@ Section WPLeaps.
 
   Variable (a: P4A.t S H).
 
-  Variable (wp: P4A.t S H ->
-                conf_rel S H ->
-                list (conf_rel S H)).
+  Variable (wp: conf_rel a ->
+                list (conf_rel a)).
 
   Notation conf := (configuration (P4A.interp a)).
 
@@ -47,13 +46,13 @@ Section WPLeaps.
   Notation δ := step.
 
   Reserved Notation "R ⇝ S" (at level 10).
-  Inductive pre_bisimulation : crel S H -> crel S H -> relation conf :=
+  Inductive pre_bisimulation : crel a -> crel a -> relation conf :=
   | PreBisimulationClose:
       forall R q1 q2,
         ⟦R⟧ q1 q2 ->
         R ⇝ [] q1 q2
   | PreBisimulationSkip:
-      forall (R T: crel S H) (C: conf_rel S H) q1 q2 (H: {R ⊨ C} + {~(R ⊨ C)}),
+      forall (R T: crel a) (C: conf_rel a) q1 q2 (H: {R ⊨ C} + {~(R ⊨ C)}),
         match H with
         | left _ => True
         | _ => False
@@ -61,12 +60,12 @@ Section WPLeaps.
         R ⇝ T q1 q2 ->
         R ⇝ (C :: T) q1 q2
   | PreBisimulationExtend:
-      forall (R T: crel S H) (C: conf_rel S H) (W: crel S H) q1 q2 (H: {R ⊨ C} + {~(R ⊨ C)}),
+      forall (R T: crel a) (C: conf_rel a) (W: crel a) q1 q2 (H: {R ⊨ C} + {~(R ⊨ C)}),
         match H with
         | right _ => True
         | _ => False
         end ->
-        W = wp a C ->
+        W = wp C ->
         (C :: R) ⇝ (W ++ T) q1 q2 ->
         R ⇝ (C :: T) q1 q2
   where "R ⇝ S" := (pre_bisimulation R S).
@@ -77,40 +76,39 @@ Section WPLeaps.
     | Datatypes.S n => range n ++ [n]
     end.
 
-  Definition not_accept1 (a: P4A.t S H) (s: S) : crel S H :=
+  Definition not_accept1 (a: P4A.t S H) (s: S) : crel a :=
     List.map (fun n =>
                 {| cr_st := {| cs_st1 := {| st_state := inr true; st_buf_len := 0 |};
                                cs_st2 := {| st_state := inl s;    st_buf_len := n |} |};
                    cr_rel := BRFalse _ BCEmp |})
              (range (P4A.size a s)).
 
-  Definition not_accept2 (a: P4A.t S H) (s: S) : crel S H :=
+  Definition not_accept2 (a: P4A.t S H) (s: S) : crel a :=
     List.map (fun n =>
                 {| cr_st := {| cs_st1 := {| st_state := inl s;    st_buf_len := n |};
                                cs_st2 := {| st_state := inr true; st_buf_len := 0 |} |};
                    cr_rel := BRFalse _ BCEmp |})
              (range (P4A.size a s)).
 
-  Definition init_rel (a: P4A.t S H) : crel S H :=
+  Definition init_rel (a: P4A.t S H) : crel a :=
     List.concat (List.map (not_accept1 a) (enum S) ++
                           List.map (not_accept2 a) (enum S)).
 
-
-  Definition sum_not_accept1 (a: P4A.t (S1 + S2) H) (s: S1) : crel (S1 + S2) H :=
+  Definition sum_not_accept1 (a: P4A.t (S1 + S2) H) (s: S1) : crel a :=
     List.map (fun n =>
                 {| cr_st := {| cs_st1 := {| st_state := inl (inl s); st_buf_len := n |};
                                cs_st2 := {| st_state := inr true;    st_buf_len := 0 |} |};
                    cr_rel := BRFalse _ BCEmp |})
              (range (P4A.size a (inl s))).
 
-  Definition sum_not_accept2 (a: P4A.t (S1 + S2) H) (s: S2) : crel (S1 + S2) H :=
+  Definition sum_not_accept2 (a: P4A.t (S1 + S2) H) (s: S2) : crel a :=
     List.map (fun n =>
                 {| cr_st := {| cs_st1 := {| st_state := inr true;    st_buf_len := 0 |};
                                cs_st2 := {| st_state := inl (inr s); st_buf_len := n |} |};
                    cr_rel := BRFalse _ BCEmp |})
              (range (P4A.size a (inr s))).
 
-  Definition sum_init_rel (a: P4A.t (S1 + S2) H) : crel (S1 + S2) H :=
+  Definition sum_init_rel (a: P4A.t (S1 + S2) H) : crel a :=
     List.concat (List.map (sum_not_accept1 a) (enum S1)
                           ++ List.map (sum_not_accept2 a) (enum S2)).
   Notation "ctx , ⟨ s1 , n1 ⟩ ⟨ s2 , n2 ⟩ ⊢ b" :=
@@ -123,7 +121,7 @@ Section WPLeaps.
   Notation bfalse := (BRFalse _ _).
   Notation "a ⇒ b" := (BRImpl a b) (at level 40).
 
-  Definition not_equally_accepting (s: Reachability.state_pair S1 S2) : bool :=
+  Definition not_equally_accepting (s: Reachability.state_pair a) : bool :=
     let '(s1, s2) := s in
     match s1.(st_state), s2.(st_state) with
     | inr true, inr true => false
@@ -132,19 +130,18 @@ Section WPLeaps.
     | _, _ => false
     end.
 
-  Definition mk_rel '((s1, s2): Reachability.state_pair S1 S2)
-    : conf_rel (S1 + S2) H :=
+  Definition mk_rel '((s1, s2): Reachability.state_pair a)
+    : conf_rel a :=
     {| cr_st := {| cs_st1 := s1;
                    cs_st2 := s2 |};
        cr_ctx := BCEmp;
        cr_rel := bfalse |}.
 
-  Definition mk_partition (r: Reachability.state_pairs _ _)
-    : crel (S1 + S2) H :=
+  Definition mk_partition (r: Reachability.state_pairs a) : crel a :=
     List.map mk_rel (List.filter not_equally_accepting r).
 
   Definition mk_init (n: nat) s1 s2 :=
-    List.nodup (@conf_rel_eq_dec _ _ _ _ _)
+    List.nodup (@conf_rel_eq_dec _ _ _ _ _ a)
                (mk_partition
                   (Reachability.reachable_states a n s1 s2)).
 
@@ -165,7 +162,7 @@ Section WPLeaps.
       C q1 q2 ->
       top q1 q2.
 
-  Definition ctopbdd (C: crel S H) : Prop :=
+  Definition ctopbdd (C: crel a) : Prop :=
     forall r,
       In r C ->
       topbdd ⦇r⦈.
@@ -173,14 +170,14 @@ Section WPLeaps.
   Definition safe_wp_1bit : Prop :=
     forall C (q1 q2: conf),
       top q1 q2 ->
-      ⟦wp a C⟧ q1 q2 ->
+      ⟦wp C⟧ q1 q2 ->
       forall bit,
         ⦇C⦈ (δ q1 bit) (δ q2 bit).
 
   Definition wp_bdd :=
-    forall a C,
+    forall C,
       topbdd ⦇C⦈ ->
-      ctopbdd (wp a C).
+      ctopbdd (wp C).
 End WPLeaps.
 Arguments pre_bisimulation {S1 equiv0 S1_eq_dec S2 equiv1 S2_eq_dec H H_eq_dec} a wp.
 
